completed unary/binary operator rules

xtext/org.archware.sosadl/src/org/archware/sosadl/validation/BinaryTypeInfo.java
@@ -19,11 +19,13 @@ public class BinaryTypeInfo<L extends DataType, R extends DataType, X extends Da
 	public final Supplier<R> rIfNone;
 	public final HeptaFunction<Environment, BinaryExpression, Pair<Type_expression, DataType>, Pair<Subtype, L>, Pair<Type_expression, DataType>, Pair<Subtype, R>, X, Type_expression_node> createProofTerm;
 	public final HexaFunction<Environment, BinaryExpression, Pair<Type_expression, DataType>, Pair<Subtype, L>, Pair<Type_expression, DataType>, Pair<Subtype, R>, X> createType;
+	public final Supplier<X> createDefault;
 
 	public BinaryTypeInfo(String operator, Class<L> lClass, String lLabel, Supplier<L> lIfNone, Class<R> rClass,
 			String rLabel, Supplier<R> rIfNone,
 			HeptaFunction<Environment, BinaryExpression, Pair<Type_expression, DataType>, Pair<Subtype, L>, Pair<Type_expression, DataType>, Pair<Subtype, R>, X, Type_expression_node> createProofTerm,
-			HexaFunction<Environment, BinaryExpression, Pair<Type_expression, DataType>, Pair<Subtype, L>, Pair<Type_expression, DataType>, Pair<Subtype, R>, X> createType) {
+			HexaFunction<Environment, BinaryExpression, Pair<Type_expression, DataType>, Pair<Subtype, L>, Pair<Type_expression, DataType>, Pair<Subtype, R>, X> createType,
+			Supplier<X> createDefault) {
 		super();
 		this.operator = operator;
 		this.lClass = lClass;
@@ -34,6 +36,7 @@ public class BinaryTypeInfo<L extends DataType, R extends DataType, X extends Da
 		this.rIfNone = rIfNone;
 		this.createProofTerm = createProofTerm;
 		this.createType = createType;
+		this.createDefault = createDefault;
 	}
 
 	public String getOperator() {
