types/coq/SosADL/Properties.v
@@ -1,0 +1,140 @@
+Require Import List.
+Require Import String.
+Require SosADL.SosADL.
+Require Import SosADL.Environment.
+Require Import SosADL.Utils.
+Require Import SosADL.Interpretation.
+Require Import SosADL.TypeSystem.
+Require Import BinInt.
+Require Import Omega.
+Require Import ZArith.
+Require Import ZArith.Zquot.
+
+
+Local Open Scope list_scope.
+Local Open Scope string_scope.
+
+Lemma interpInZ_implies_constexpr: forall e f (H: interp_in_Z e = Interpreted f), expression e is constant integer.
+Proof.
+  intros.
+  assert (exists f, interp_in_Z e = Interpreted f) as I by (exists f; auto).
+  clear f H.
+  revert e I.
+  apply interp_in_Z_ind; intros; constructor; auto.
+Qed.
+
+Ltac Zbool_to_cmp :=
+  repeat match goal with
+         | H: ((_ <=? _)%Z = true) |- _ => apply Zbool.Zle_bool_imp_le in H
+         end.
+
+Ltac interp_to_Zle :=
+  repeat match goal with
+         | H: (_ <= _) |- _ => inversion H; subst; clear H
+         end;
+  repeat match goal with
+         | H1: (interp_in_Z ?e = Interpreted ?f),
+               H2: (interp_in_Z ?e = Interpreted ?g) |- _ =>
+           rewrite H1 in H2; inversion H2; subst; clear H2
+         end.
+
+Ltac auto_rewrite :=
+  simpl;
+  repeat match goal with
+         | H: (?x = _) |- _ => rewrite H
+         end;
+  auto.
+
+Lemma range_modulo_min_ok: forall lmin l lmax rmin r rmax min
+                                  (H1: range_modulo_min lmin lmax rmin rmax min)
+                                  (H2: lmin <= l)
+                                  (H3: l <= lmax)
+                                  (H4: rmin <= r)
+                                  (H5: r <= rmax),
+    min <= (SosADL.SosADL.BinaryExpression (Some l) (Some "mod") (Some r)).
+Proof.
+  intros.
+  interp_to_Zle.
+  Zbool_to_cmp.
+  destruct H1.
+  - interp_to_Zle.
+    assert (zr3 = (1 - zr)%Z) by (unfold interp_in_Z in *; rewrite p2 in p13; inversion p13; auto).
+    subst. clear p13.
+    inversion p10. subst. clear p10.
+    apply In_Z with (zl := zl) (zr := Z.rem zr2 zr0).
+    + auto.
+    + auto_rewrite.
+    + apply Zbool.Zle_imp_le_bool.
+      Zbool_to_cmp.
+      assert ((0 < zr0)%Z) by omega.
+      destruct (Z.le_ge_cases zr2 0%Z).
+      * generalize (Zrem_lt_neg_pos _ _ H0 H). omega.
+      * generalize (Zrem_lt_pos_pos _ _ H0 H). omega.
+  - interp_to_Zle. Zbool_to_cmp.
+    apply In_Z with (zl := zl) (zr := (Z.rem zr2 zr0)).
+    + auto.
+    + auto_rewrite.
+    + apply Zbool.Zle_imp_le_bool.
+      inversion p13. subst. clear p13.
+      assert ((0 <= zr2)%Z) by omega.
+      Zquot.zero_or_not zr0.
+      generalize (Zquot.Zrem_lt_pos _ _ H H0).
+      omega.
+  - interp_to_Zle. Zbool_to_cmp.
+    apply In_Z with (zl := zl) (zr := (Z.rem zr2 zr0)).
+    + auto.
+    + auto_rewrite.
+    + apply Zbool.Zle_imp_le_bool.
+      inversion p13. rewrite p0 in H0. inversion H0. subst. clear H0 p13.
+      inversion p15. subst. clear p15.
+      assert ((zr0 < 0)%Z) by omega.
+      destruct (Z.le_ge_cases zr2 0%Z).
+      * generalize (Zrem_lt_neg_neg _ _ H0 H). omega.
+      * generalize (Zrem_lt_pos_neg _ _ H0 H). omega.
+Qed.
+
+Lemma range_modulo_max_ok: forall lmin l lmax rmin r rmax max
+                                  (H1: range_modulo_max lmin lmax rmin rmax max)
+                                  (H2: lmin <= l)
+                                  (H3: l <= lmax)
+                                  (H4: rmin <= r)
+                                  (H5: r <= rmax),
+    (SosADL.SosADL.BinaryExpression (Some l) (Some "mod") (Some r)) <= max.
+Proof.
+  intros.
+  interp_to_Zle.
+  Zbool_to_cmp.
+  destruct H1.
+  - interp_to_Zle. Zbool_to_cmp.
+    inversion p12. rewrite p2 in H0. inversion H0. subst. clear p12 H0.
+    inversion p10. subst. clear p10.
+    apply In_Z with (zl := Z.rem zr2 zr0) (zr := zr3).
+    + auto_rewrite.
+    + auto.
+    + apply Zbool.Zle_imp_le_bool.
+      assert ((0 < zr0)%Z) by omega.
+      destruct (Z.le_ge_cases zr2 0%Z).
+      * generalize (Zrem_lt_neg_pos _ _ H0 H). omega.
+      * generalize (Zrem_lt_pos_pos _ _ H0 H). omega.
+  - interp_to_Zle. Zbool_to_cmp.
+    apply In_Z with (zl := (Z.rem zr2 zr0)) (zr := zr3).
+    + auto_rewrite.
+    + auto.
+    + apply Zbool.Zle_imp_le_bool.
+      inversion p12. subst. clear p12.
+      assert ((zr2 <= 0)%Z) by omega.
+      Zquot.zero_or_not zr0.
+      generalize (Zquot.Zrem_lt_neg _ _ H H0).
+      omega.
+  - interp_to_Zle. Zbool_to_cmp.
+    assert (zl = (1 - zl0)%Z) by (unfold interp_in_Z in *; rewrite p0 in p12; inversion p12; auto). subst. clear p12.
+    inversion p15. subst. clear p15.
+    apply In_Z with (zl := (Z.rem zr2 zr0)) (zr := zr3).
+    + auto_rewrite.
+    + auto.
+    + apply Zbool.Zle_imp_le_bool.
+      assert ((zr0 < 0)%Z) by omega.
+      destruct (Z.le_ge_cases zr2 0%Z).
+      * generalize (Zrem_lt_neg_neg _ _ H0 H). omega.
+      * generalize (Zrem_lt_pos_neg _ _ H0 H). omega.
+Qed.
