types/coq/make-allpdf.sh
@@ -1,3 +1,4 @@
 #!/bin/sh
 
+rm all.pdf
 make -j2 && make 'COQDOCLIBS=-p "\usepackage{listings}"' all.pdf
